Automata/NFA/Pumping.lean
@@ -1,0 +1,99 @@
+import Automata.NFA.Basic
+import Automata.NFA.Trace
+
+namespace NFA
+variable (m : NFA α)
+
+theorem php [Fin.Enum α] (f : Nat → α) : ∃ i j, i < j ∧ j ≤ Fin.Enum.size α ∧ f i = f j := by sorry
+
+theorem pumping (n : Nat) :
+  m.run xs s t → m.run ys t t → m.run zs t u → m.run (xs ++ ys.rep n ++ zs) s u := by
+  induction n using Nat.recAux generalizing xs ys zs with
+  | zero =>
+    intro hx _ hz
+    rw [List.rep]
+    rw [List.append_nil]
+    rw [m.run_append]
+    exists t
+  | succ n ih =>
+    intro hx hy hz
+    rw [List.rep_succ]
+    rw [List.append_assoc]
+    rw [List.append_assoc]
+    rw [← List.append_assoc]
+    apply ih
+    · exact hx
+    · exact hy
+    · rw [m.run_append]
+      exists t
+
+@[simp] theorem splitting [Fin.Enum  α] : ws.length ≥ m.size → m.run ws s t → ∃ (u : m.State) (xs ys zs : List α), ws = xs ++ ys ++ zs ∧ ys.length > 0 ∧ m.run xs s u ∧ m.run ys u u ∧ m.run zs u t := by
+  intro hw hrun
+  match m.trace_of_run hrun with
+  | ⟨p, hp⟩ =>
+    match php p.val with
+    | ⟨i,j,hij,hjs,hval⟩ =>
+      let zs := ws.drop j
+      let ys := (ws.take j).drop i
+      let xs := (ws.take j).take i
+      let pz := p.drop j
+      let py := (p.take j).drop i
+      let px := (p.take j).take i
+      have hz : Trace m zs pz := m.trace_drop j hp
+      have hy : Trace m ys py := m.trace_drop i (m.trace_take j hp)
+      have hx : Trace m xs px := m.trace_take i (m.trace_take j hp)
+      have hjp : j ≤ p.length := by
+        rw [←Trace.length_eq_length m hp]
+        transitivity m.size
+        · exact hjs
+        · exact hw
+      have hpij : p.val i = (p.take j).val i := by rw [Path.val_take hjp (Nat.le_of_lt hij)]
+      exists p.val i, xs, ys, zs
+      constructor
+      · calc
+        _ = ws.take j ++ zs := by rw [List.take_append_drop j]
+        _ = (xs ++ ys) ++ zs := by rw [List.take_append_drop i]
+      · constructor
+        · have : j ≤ ws.length := Nat.le_trans hjs hw
+          rw [List.length_drop i (ws.take j)]
+          rw [List.length_take j ws]
+          rw [Nat.min_eq_left this]
+          apply Nat.sub_pos_of_lt hij
+        · constructor
+          · rw [hpij]
+            apply m.run_of_trace hx
+          · constructor
+            · transitivity (m.run ys (p.val i) (p.val j))
+              · rw [hval]
+              · rw [hpij]
+                apply m.run_of_trace hy
+            · rw [hval]
+              apply m.run_of_trace hz
+
+@[simp] theorem reachableAux [Fin.Enum α] : ws.length < n → m.run ws s t → ∃ (ws : List α), ws.length < m.size ∧ m.run ws s t := by
+  intro hws hrun
+  induction n generalizing ws with
+  | zero => contradiction
+  | succ n ih =>
+    if hwslt: ws.length < m.size then
+      exists ws
+    else
+      have hge : ws.length ≥ m.size := Nat.le_of_not_lt hwslt
+      match m.splitting hge hrun with
+      | ⟨u,xs,ys,zs,heq,hys,hxrun,_,hzrun⟩ =>
+        have hrun : m.run (xs ++ zs) s t := by
+          rw [run_append]
+          exists u
+        have hlt : (xs ++ zs).length < n := calc
+          _ = xs.length + zs.length := by rw [List.length_append]
+          _ < (xs.length + ys.length) + zs.length := by apply Nat.add_lt_add_right; apply Nat.lt_add_of_pos_right; exact hys
+          _ = (xs ++ ys).length + zs.length := by rw [List.length_append]
+          _ = ((xs ++ ys) ++ zs).length := by rw [List.length_append (xs ++ ys)]
+          _ = ws.length := by rw [heq]
+          _ ≤ n := by apply Nat.le_of_lt_succ hws
+        apply ih hlt hrun
+
+@[simp] theorem reachable [Fin.Enum α] : m.run ws s t → ∃ (ws : List α), ws.length < m.size ∧ m.run ws s t :=
+  m.reachableAux (Nat.lt_succ_self ws.length)
+
+end NFA
